theories/simulations/msim/Tactics.v
@@ -9,32 +9,70 @@ Tactic Notation "iwcase" tactic(itac) tactic(wtac) :=
   | [ |- environments.envs_entails _ (wsim _ _ _ _ _ _ _ _ _ _ _ _ _) ] => wtac
   end.
 
-Ltac cStepS := iwcase (do 1 istep_s) (do 1 wstep_s).
-Ltac cStepsS := iwcase (do 1 isteps_s) (do 1 wsteps_s).
+Ltac dStepS := cShowS; iwcase (do 1 istep_s) (do 1 wstep_s).
+Ltac cStepS := dStepS; cHideS.
+Ltac dStepsS := cShowS; iwcase (do 1 isteps_s) (do 1 wsteps_s).
+Ltac cStepsS := dStepsS; cHideS.
 
-Ltac cStepT := iwcase (do 1 istep_t) (do 1 wstep_t).
-Ltac cStepsT := iwcase (do 1 isteps_t) (do 1 wsteps_t).
+Ltac dStepT := cShowT; iwcase (do 1 istep_t) (do 1 wstep_t).
+Ltac cStepT := dStepT; cHideT.
+Ltac dStepsT := cShowT; iwcase (do 1 isteps_t) (do 1 wsteps_t).
+Ltac cStepsT := dStepsT; cHideT.
 
-Tactic Notation "cStep" ident(name) := iwcase (do 1 istep name) (do 1 wstep name).
-Tactic Notation "cStep" := iwcase (do 1 istep) (do 1 wstep).
+Tactic Notation "dStep" := cShowS; cShowT; iwcase (do 1 istep) (do 1 wstep).
+Tactic Notation "cStep" := dStep; cHideS; cHideT.
 
-Tactic Notation "cForceS" := iwcase (do 1 iforce_s) (do 1 wforce_s).
-Tactic Notation "cForceS" uconstr(p) := iwcase (do 1 iforce_s p) (do 1 wforce_s p).
-Ltac cForcesS := iwcase (do 1 iforces_s) (do 1 wforces_s).
+Tactic Notation "dStep" ident(name) := cShowS; cShowT; iwcase (do 1 istep name) (do 1 wstep name).
+Tactic Notation "cStep" ident(name) := dStep name; cHideS; cHideT.
 
-Tactic Notation "cForceT" := iwcase (do 1 iforce_t) (do 1 wforce_t).
-Tactic Notation "cForceT" uconstr(p) := iwcase (do 1 iforce_t p) (do 1 wforce_t p).
-Ltac cForcesT := iwcase (do 1 iforces_t) (do 1 wforces_t).
+Tactic Notation "dForceS" := cShowS; iwcase (do 1 iforce_s) (do 1 wforce_s).
+Tactic Notation "cForceS" := dForceS; cHideS.
 
-Ltac cInlineS := iwcase (do 1 iinline_s) (do 1 winline_s).
-Ltac cInlineT := iwcase (do 1 iinline_t) (do 1 winline_t).
+Tactic Notation "dForceS" uconstr(p) := cShowS; iwcase (do 1 iforce_s p) (do 1 wforce_s p).
+Tactic Notation "cForceS" uconstr(p) := dForceS p; cHideS.
 
-Ltac cCall hyps := iwcase (do 1 icall hyps) (do 1 wcall hyps).
-Ltac cYield hyps := iwcase (do 1 iyield hyps) (do 1 wyield hyps).
+Ltac dForcesS := cShowS; iwcase (do 1 iforces_s) (do 1 wforces_s).
+Ltac cForcesS := dForcesS; cHideS.
+
+Tactic Notation "dForceT" := cShowT; iwcase (do 1 iforce_t) (do 1 wforce_t).
+Tactic Notation "cForceT" := dForceT; cHideT.
+
+Tactic Notation "dForceT" uconstr(p) := cShowT; iwcase (do 1 iforce_t p) (do 1 wforce_t p).
+Tactic Notation "cForceT" uconstr(p) := dForceT p; cHideT.
+
+Ltac dForcesT := cShowT; iwcase (do 1 iforces_t) (do 1 wforces_t).
+Ltac cForcesT := dForcesT; cHideT.
+
+Ltac dInlineS := cShowS; iwcase (do 1 iinline_s) (do 1 winline_s).
+Ltac cInlineS := dInlineS; cHideS.
+
+Ltac dInlineT := cShowT; iwcase (do 1 iinline_t) (do 1 winline_t).
+Ltac cInlineT := dInlineT; cHideT.
+
+Tactic Notation "dCall" uconstr(hyps) "as" "(" simple_intropattern(vret) simple_intropattern(st_src) simple_intropattern(st_tgt) ")" uconstr(IST) :=
+  cShowS; cShowT; iwcase (do 1 icall hyps as (vret st_src st_tgt) IST) (do 1 wcall hyps as (vret st_src st_tgt) IST).
+Tactic Notation "cCall" uconstr(hyps) "as" "(" simple_intropattern(vret) simple_intropattern(st_src) simple_intropattern(st_tgt) ")" uconstr(IST) :=
+  dCall hyps as (vret st_src st_tgt) IST; cHideS; cHideT.
+
+Tactic Notation "dYield" uconstr(hyps) "as" "(" simple_intropattern(st_src) simple_intropattern(st_tgt) ")" uconstr(IST) :=
+  cShowS; cShowT; iwcase (do 1 iyield hyps as (st_src st_tgt) IST) (do 1 wyield hyps as (st_src st_tgt) IST).
+Tactic Notation "cYield" uconstr(hyps) "as" "(" simple_intropattern(st_src) simple_intropattern(st_tgt) ")" uconstr(IST) :=
+  dYield hyps as (st_src st_tgt) IST; cHideS; cHideT.
 
 Ltac cByCoind CIH := iwcase (do 1 iby_coind CIH) (do 1 wby_coind CIH).
 
-Tactic Notation "cBind" uconstr(RR) := iwcase (do 1 ibind RR) (do 1 wbind RR).
+Tactic Notation "dBind" uconstr(RR) "as" "(" simple_intropattern(st_s) simple_intropattern(r_s) simple_intropattern(st_t) simple_intropattern(r_t) ")" uconstr(Q) :=
+  cShowS; cShowT; iwcase (do 1 ibind RR as (st_s r_s st_t r_t) Q) (do 1 wbind RR as (st_s r_s st_t r_t) Q).
+Tactic Notation "cBind" uconstr(RR) "as" "(" simple_intropattern(st_s) simple_intropattern(r_s) simple_intropattern(st_t) simple_intropattern(r_t) ")" uconstr(Q) :=
+  dBind RR as (st_s r_s st_t r_t) Q; cHideS; cHideT.
+
+Tactic Notation "dBind" uconstr(RR) uconstr(hyps) "as" "(" simple_intropattern(st_s) simple_intropattern(r_s) simple_intropattern(st_t) simple_intropattern(r_t) ")" uconstr(Q) :=
+  cShowS; cShowT; iwcase (do 1 ibind RR hyps as (st_s r_s st_t r_t) Q) (do 1 wbind RR hyps as (st_s r_s st_t r_t) Q).
+Tactic Notation "cBind" uconstr(RR) uconstr(hyps) "as" "(" simple_intropattern(st_s) simple_intropattern(r_s) simple_intropattern(st_t) simple_intropattern(r_t) ")" uconstr(Q) :=
+  dBind RR hyps as (st_s r_s st_t r_t) Q; cHideS; cHideT.
+
+Tactic Notation "cIst" constr(IST) "with" constr(H) :=
+  iwcase (do 1 iIst IST with H) (do 1 wIst IST with H).
 
 Ltac _clear_ibot H :=
   let ty := type of H in
@@ -80,7 +118,6 @@ Tactic Notation "cCoind" ident(CIH) ident(g) ident(LEg) "with" ident(id5) ident(
   first [eapply wsim_coind | eapply isim_coind];
   intros g LEg CIH [id5 [id4 [id3 [id2 id1]]]];
   s; destruct_quant CIH; _clear_ibot LEg.
-
 
 Tactic Notation "cCoind" ident(CIH) ident(g) ident(LEg) "with" ident(id6) ident(id5) ident(id4) ident(id3) ident(id2) ident(id1) :=
   iStopProof;
